% hh
因为

\begin{align*}
	\hat{l}_{\mathrm{z}}\varphi _m=m\hbar \varphi _m\\
	\left[ l_x,l_y \right] =i\hbar l_z\\
	\left[ l_y,l_z \right] =i\hbar l_x\\
	i\hbar \hat{l}_x=\hat{l}_y\hat{l}_z-\hat{l}_z\hat{l}y\\
	i\hbar \left. \langle m\left| \hat{l}_x \right|m \right. \rangle =\langle m|\left( \hat{l}y\left| \hat{l}_z \right|m \right. \rangle -\left. \langle m\left| \hat{l}_z\hat{l}_y \right|m \right. \rangle\\
	i\hbar \vec{l}_x=m\hbar \langle m|\hat{l}|m\rangle -m\hbar \left. \langle m\left| \hat{l}_y \right|m \right. \rangle =\\
	L_x=0\\
\end{align*}