% hh
因为

对于$\hat{l}_x$，因为
$$
i\hbar l_x=\left[ l_y,l_z \right] =\hat{l}_y\hat{l}_z-\hat{l}_z\hat{l}_y
$$
两边对|m$\rangle$求平均值
\begin{align}
i\hbar \left. \langle m|\hat{l}_x|m \right. \rangle &=\langle m|\hat{l}_y\hat{l}_z|m\rangle -\left. \langle m\left| \hat{l}_z\hat{l}_y \right|m \right. \rangle\\
	i\hbar \bar{l}_x&=m\hbar \langle m|\hat{l}_y|m\rangle -m\hbar \left. \langle m|\hat{l}_y|m \right. \rangle \\
	\bar{l}_x&=0
\end{align}

同理对于$\hat{l}_x$，因为
$$
i\hbar l_y=\left[ l_y,l_z \right] =\hat{l}_y\hat{l}_z-\hat{l}_z\hat{l}_y
$$
两边对|m$\rangle$求平均值
\begin{align}
i\hbar \left. \langle m|\hat{l}_x|m \right. \rangle &=\langle m|\hat{l}_y\hat{l}_z|m\rangle -\left. \langle m\left| \hat{l}_z\hat{l}_y \right|m \right. \rangle\\
	i\hbar \bar{l}_x&=m\hbar \langle m|\hat{l}_y|m\rangle -m\hbar \left. \langle m|\hat{l}_y|m \right. \rangle \\
	\bar{l}_x&=0
\end{align}